\subsection{Sinsemilla Hash}

We use Halo2 \cite{website:halo2} Sinsemilla Hash scheme.

For detailed design of the hash algorithm and the parameters used below, please refer to Section \ref{sec:key-technologies}.
Following is the main calculation process of Sinsemilla:
\begin{enumerate}
    \item Set the initial value $\mathrm{Acc}_0 = Q$
    \item Perform loop calculation of $i$ from $0$ to $n-1$:
    \[ \mathrm{Acc}_{i+1} = (\mathrm{Acc}_i + P_{m_{i+1}}) + \mathrm{Acc}_i. \]
\end{enumerate}

Now, let $R_i = \mathrm{Acc}_i + P_{m_{i+1}}$, then $\mathrm{Acc}_{i+1} = R_i + \mathrm{Acc}_i$ then according to previous definition, we have
\begin{align*}
\lambda_{1,i} &= \frac {y_{Acc,i} - y_{P,i}}{x_{Acc,i}-x_{P,i}}, \\
x_{R,i} &= \lambda_{1,i}^2 - x_{\text{Acc},i}-x_{P,i}, \\
y_{R,i} &= \lambda_{1,i} (x_{\text{Acc},i} - x_{R,i}) - y_{\text{Acc},i}, \\
\lambda_{2,i} &= \frac {y_{\text{Acc},i} - y_{R,i}}{x_{\text{Acc},i}-x_{R,i}}, \\
x_{\text{Acc},i+1} &= \lambda_{2,i}^2 - x_{\text{Acc},i}-x_{R,i}, \\
y_{\text{Acc},i+1} &= \lambda_{2,i} (x_{\text{Acc},i} - x_{\text{Acc},i+1}) - y_{\text{Acc},i}.
\end{align*}

So, we have constrains as in Table \ref{table:raw-sinsemilla-hash-constraints}.
\begin{table}[!ht]
    \centering
    \begin{tabular}{|c|l|l|}
    \hline
    \emph{Degree} & \emph{Constraints} & \emph{Notes} \\
    \hline
    3 & $q_\text{incomplete-add} \cdot (x_{R,i} + x_{\text{Acc},i} + x_{P,i} - \lambda_{1,i}^2) = 0$
    & $x_{R,i} = \lambda_{1,i}^2 - x_{\text{Acc},i} - x_{P,i}$ \\
    3 & $q_\text{incomplete-add} \cdot (\lambda_{1,i} (x_{\text{Acc},i} - x_{R,i}) - (y_{\text{Acc},i} + y_{R,i})) = 0$
    & $y_{R,i} = \lambda_{1,i} (x_{\text{Acc},i} - x_{R,i}) - y_{\text{Acc},i}$ \\
    3 & $q_\text{incomplete-add} \cdot (\lambda_{1,i} (x_{\text{Acc},i} - x_{P,i}) - (y_{\text{Acc},i} - y_{P,i})) = 0$
    & $\lambda_{1,i} = (y_{\text{Acc},i} - y_{P,i}) / (x_{\text{Acc},i}-x_{P,i})$ \\
    3 & $q_\text{incomplete-add} \cdot (x_{\text{Acc},i+1} + x_{\text{Acc},i} + x_{R,i} - \lambda_{2,i}^2) = 0$
    & $x_{\text{Acc},i+1} = \lambda_{2,i}^2 - x_{\text{Acc},i}-x_{R,i}$ \\
    3 & $q_\text{incomplete-add} \cdot (\lambda_{2,i} (x_{\text{Acc},i} - x_{\text{Acc},i+1}) - (y_{\text{Acc},i} + y_{\text{Acc},i+1})) = 0$
    & $y_{\text{Acc},i+1} = \lambda_{2,i} (x_{\text{Acc}_,i} - x_{\text{Acc},i+1}) - y_{\text{Acc},i}$ \\
    3 & $q_\text{incomplete-add} \cdot (\lambda_{2,i} (x_{\text{Acc},i} - x_{R,i}) - (y_{\text{Acc},i} - y_{R,i}) ) = 0$
    & $\lambda_{2,i} = (y_{\text{Acc},i} - y_{R,i}) / (x_{\text{Acc}_i}-x_{R,i})$ \\
    \hline
    \end{tabular}
    \caption{Sinsemilla Hash constraints}
    \label{table:raw-sinsemilla-hash-constraints}
\end{table}
\begin{align*}
    & \lambda_{2,i} = \frac {y_{\text{Acc},i} - y_{R,i}}{x_{\text{Acc},i}-x_{R,i}} \\
    \implies & y_{\text{Acc},i} - y_{R,i} = \lambda_{2,i} (x_{\text{Acc},i}-x_{R,i}), \\
    & y_{R,i} = \lambda_{1,i} (x_{\text{Acc},i} - x_{R,i}) - y_{\text{Acc},i} \\
    \implies & y_{\text{Acc},i} - (\lambda_{1,i} (x_{\text{Acc},i} - x_{R,i}) - y_{\text{Acc},i}) = \lambda_{2,i} (x_{\text{Acc},i}-x_{R,i}) \\
    \implies & 2y_{\text{Acc},i} = (\lambda_{1,i} + \lambda_{2,i}) (x_{\text{Acc},i}-x_{R,i}).
\end{align*}

Therefore, the check for $\lambda_{2,i} = (y_{\text{Acc}_i} - y_{R,i})/(x_{\text{Acc}_i}-x_{R,i})$ can be replaced by
\[ q_\text{incomplete-add} \cdot (\lambda_{2,i} (x_{\text{Acc},i} - x_{R,i}) - (y_{\text{Acc},i} - y_{R,i}) ) = 0, \]

then
\[ q_\text{incomplete-add} \cdot ((\lambda_{2,i} + \lambda_{1,i}) (x_{\text{Acc},i} - x_{R,i}) - 2y_{\text{Acc},i}) = 0. \]

We haven't used $y_{R,i}$ of $R_i = \{x_{R,i}, y_{R,i}\}$ in the second step of checking for $\mathrm{Acc}_{i+1} = R_i + \mathrm{Acc}_i$. Therefore, remove the constraint on $y_{R,i}$ in the first step and the entire constraint develop into what is displayed in Table \ref{table:simplified-sinsemilla-hash-constraints}.

\begin{table}[!ht]
    \centering
    \begin{tabular}{|c|l|l|}
        \hline
        \emph{Degree} & \emph{Constraints} & \emph{Notes} \\
        \hline
        3 & $q_\text{incomplete-add} \cdot (x_{R,i} + x_{\text{Acc},i} + x_{P,i} - \lambda_{1,i}^2) = 0$
        & $x_{R,i} = \lambda_{1,i}^2 - x_{\text{Acc},i} - x_{P,i}$ \\
        3 & $q_\text{incomplete-add} \cdot (\lambda_{1,i} (x_{\text{Acc},i} - x_{P,i}) - (y_{\text{Acc},i} - y_{P,i})) = 0$
        & $\lambda_{1,i} = (y_{\text{Acc},i} - y_{P,i}) / (x_{\text{Acc},i}-x_{P,i})$ \\
        3 & $q_\text{incomplete-add} \cdot (x_{\text{Acc},i+1} + x_{\text{Acc},i} + x_{R,i} - \lambda_{2,i}^2) = 0$
        & $x_{\text{Acc},i+1} = \lambda_{2,i}^2 - x_{\text{Acc},i}-x_{R,i}$ \\
        3 & $q_\text{incomplete-add} \cdot (\lambda_{2,i} (x_{\text{Acc},i} - x_{\text{Acc},i+1}) - (y_{\text{Acc},i} + y_{\text{Acc},i+1})) = 0$
        & $y_{\text{Acc},i+1} = \lambda_{2,i} (x_{\text{Acc},i} - x_{\text{Acc},i+1}) - y_{\text{Acc},i}$ \\
        3 & $q_\text{incomplete-add} \cdot ((\lambda_{2,i} + \lambda_{1,i}(x_{\text{Acc},i} - x_{R,i}) - 2y_{\text{Acc},i} ) = 0$
        & $\lambda_{2,i} = (y_{\text{Acc},i} - y_{R,i}) / (x_{\text{Acc},i}-x_{R,i})$ \\
        \hline
    \end{tabular}
    \caption{Simplified Sinsemilla Hash constraints}
    \label{table:simplified-sinsemilla-hash-constraints}
\end{table}
